lib/concurrency/examples/Plus2_Prefix.thy
@@ -12,44 +12,46 @@ begin
 section \<open>The plus2 example.\<close>
 
 text \<open>
-This example presents an application of prefix refinement
-to solve the plus2 verification problem.
+  This example presents an application of prefix refinement
+  to solve the plus2 verification problem.
 
-The function below can be proven to do two increments per
-instance when grouped in parallel. But RG-reasoning doesn't
-work well for this proof, since the state change (+1) performed
-by the counterparts must be allowed by the rely, which must be
-transitively closed, allowing any number of (+1) operations,
-which is far too general.
+  The function below can be proven to do two increments per
+  instance when grouped in parallel. But RG-reasoning doesn't
+  work well for this proof, since the state change (+1) performed
+  by the counterparts must be allowed by the rely, which must be
+  transitively closed, allowing any number of (+1) operations,
+  which is far too general.
 
-We address the issue with a ghost variable which records the number
-of increments by each thread. We use prefix refinement to relate the
-program with ghost variable to the initial program.
-\<close>
+  We address the issue with a ghost variable which records the number
+  of increments by each thread. We use prefix refinement to relate the
+  program with ghost variable to the initial program.\<close>
 
 definition
-  "plus2 \<equiv> do env_steps; modify ((+) (1 :: nat));
-    interference; modify ((+) 1); interference od"
+  "plus2 \<equiv> do
+     env_steps;
+     modify ((+) (1 :: nat));
+     interference;
+     modify ((+) 1);
+     interference
+   od"
 
 section \<open>The ghost-extended program.\<close>
 
-record
-  plus2_xstate =
-    mainv :: nat
-    threadv :: "nat \<Rightarrow> nat"
+record plus2_xstate =
+  mainv :: nat
+  threadv :: "nat \<Rightarrow> nat"
 
-definition
-  point_update :: "'a \<Rightarrow> ('b \<Rightarrow> 'b) \<Rightarrow> (('a \<Rightarrow> 'b) \<Rightarrow> ('a \<Rightarrow> 'b))"
-where
+definition point_update :: "'a \<Rightarrow> ('b \<Rightarrow> 'b) \<Rightarrow> (('a \<Rightarrow> 'b) \<Rightarrow> ('a \<Rightarrow> 'b))" where
   "point_update x fup f = f (x := fup (f x))"
 
 definition
-  "plus2_x tid \<equiv> do env_steps;
-    modify (mainv_update ((+) 1) o threadv_update (point_update tid ((+) 1)));
-    interference;
-    modify (mainv_update ((+) 1) o threadv_update (point_update tid ((+) 1)));
-    interference
-  od"
+  "plus2_x tid \<equiv> do
+     env_steps;
+     modify (mainv_update ((+) 1) o threadv_update (point_update tid ((+) 1)));
+     interference;
+     modify (mainv_update ((+) 1) o threadv_update (point_update tid ((+) 1)));
+     interference
+   od"
 
 section \<open>Verifying the extended @{term plus2}.\<close>
 text \<open>The RG-reasoning needed to verify the @{term plus2_x} program.\<close>
@@ -57,8 +59,8 @@ definition
   "plus2_inv tids s = (mainv s = sum (threadv s) tids)"
 
 definition
-  "plus2_rel tids fix_tids s0 s
-    = ((plus2_inv tids s0 \<longrightarrow> plus2_inv tids s) \<and> (\<forall>tid \<in> fix_tids. threadv s tid = threadv s0 tid))"
+  "plus2_rel tids fix_tids s0 s =
+     ((plus2_inv tids s0 \<longrightarrow> plus2_inv tids s) \<and> (\<forall>tid \<in> fix_tids. threadv s tid = threadv s0 tid))"
 
 lemma plus2_rel_trans[simp]:
   "rtranclp (plus2_rel tids ftids) = plus2_rel tids ftids"
@@ -68,16 +70,17 @@ lemma plus2_rel_trans[simp]:
   done
 
 lemma plus2_inv_Suc[simp]:
-  "tid \<in> tids \<Longrightarrow> finite tids
-    \<Longrightarrow> plus2_inv tids (mainv_update Suc (threadv_update (point_update tid Suc) s))
-        = plus2_inv tids s"
+  "\<lbrakk>tid \<in> tids; finite tids\<rbrakk>
+   \<Longrightarrow> plus2_inv tids (mainv_update Suc (threadv_update (point_update tid Suc) s))
+       = plus2_inv tids s"
   apply (simp add: plus2_inv_def point_update_def)
   apply (simp add: sum.If_cases[where h=f and g=f and P="(=) tid" and A="tids" for f x, simplified])
   done
 
 theorem plus2_x_property:
   "\<lbrace>\<lambda>s0 s. plus2_inv tids s \<and> threadv s tid = 0 \<and> s = s0 \<and> tid \<in> tids \<and> finite tids\<rbrace>,\<lbrace>plus2_rel tids {tid}\<rbrace>
-    plus2_x tid \<lbrace>plus2_rel tids (- {tid})\<rbrace>,\<lbrace>\<lambda>_ _ s. plus2_inv tids s \<and> threadv s tid = 2\<rbrace>"
+   plus2_x tid
+   \<lbrace>plus2_rel tids (- {tid})\<rbrace>,\<lbrace>\<lambda>_ _ s. plus2_inv tids s \<and> threadv s tid = 2\<rbrace>"
   apply (simp add: plus2_x_def)
   apply wpsimp
   apply (clarsimp simp: plus2_rel_def point_update_def)
@@ -85,7 +88,8 @@ theorem plus2_x_property:
 
 corollary plus2_x_parallel:
   "\<lbrace>\<lambda>s0 s. mainv s = 0 \<and> (\<forall>tid \<in> {1, 2}. threadv s tid = 0) \<and> s = s0\<rbrace>,\<lbrace>\<lambda>a b. a = b\<rbrace>
-    parallel (plus2_x 1) (plus2_x 2) \<lbrace>\<lambda>s0 s. True\<rbrace>,\<lbrace>\<lambda>_ s0 s. mainv s = 4\<rbrace>"
+   parallel (plus2_x 1) (plus2_x 2)
+   \<lbrace>\<lambda>s0 s. True\<rbrace>,\<lbrace>\<lambda>_ s0 s. mainv s = 4\<rbrace>"
   apply (rule rg_weaken_pre)
    apply (rule rg_strengthen_post)
     apply ((rule rg_validI plus2_x_property[where tids="{1, 2}"])+; simp add: plus2_rel_def le_fun_def)
@@ -94,8 +98,7 @@ corollary plus2_x_parallel:
   done
 
 section \<open>Mapping across prefix refinement.\<close>
-text \<open>Proving prefix refinement of @{term plus2} and @{term plus2_x} and
-deriving the final result.\<close>
+text \<open>Proving prefix refinement of @{term plus2} and @{term plus2_x} and deriving the final result.\<close>
 
 lemma env_stable:
   "env_stable AR R (\<lambda>s t. t = mainv s) (\<lambda>s t. t = mainv s) \<top>"
@@ -103,9 +106,9 @@ lemma env_stable:
   apply (simp add: plus2_xstate.splits)
   done
 
-abbreviation(input)
-  "p_refn rvr P Q AR R \<equiv> prefix_refinement (\<lambda>s t. t = mainv s) (\<lambda>s t. t = mainv s)
-    (\<lambda>s t. t = mainv s) rvr P Q AR R"
+abbreviation (input)
+  "p_refn rvr P Q AR R \<equiv>
+     prefix_refinement (\<lambda>s t. t = mainv s) (\<lambda>s t. t = mainv s) (\<lambda>s t. t = mainv s) rvr P Q AR R"
 
 theorem pfx_refn_plus2_x:
   "p_refn (\<top>\<top>) (=) (\<top>\<top>) AR R (plus2_x tid) plus2"
@@ -128,10 +131,11 @@ lemma prefix_closed_plus2:
 
 theorem plus2_parallel:
   "\<lbrace>\<lambda>s0 s. s = 0 \<and> s = s0\<rbrace>,\<lbrace>\<lambda>a b. a = b\<rbrace>
-    parallel plus2 plus2 \<lbrace>\<lambda>s0 s. True\<rbrace>,\<lbrace>\<lambda>_ s0 s. s = 4\<rbrace>"
+   parallel plus2 plus2
+   \<lbrace>\<lambda>s0 s. True\<rbrace>,\<lbrace>\<lambda>_ s0 s. s = 4\<rbrace>"
   apply (rule_tac sr="\<lambda>s t. t = mainv s" in prefix_refinement_validI)
-  apply (rule prefix_refinement_parallel_triv;
-      ((rule par_tr_fin_plus2_x prefix_closed_plus2)?))
+      apply (rule prefix_refinement_parallel_triv;
+             ((rule par_tr_fin_plus2_x prefix_closed_plus2)?))
        apply (rule pfx_refn_plus2_x[where tid=1])
       apply (rule pfx_refn_plus2_x[where tid=2])
      apply clarsimp
@@ -146,14 +150,13 @@ theorem plus2_parallel:
   done
 
 section \<open>Generalising\<close>
-text \<open>Just for fun, generalise to arbitrarily many
-copies of the @{term plus2} program.\<close>
+text \<open>Just for fun, generalise to arbitrarily many copies of the @{term plus2} program.\<close>
 
 lemma plus2_x_n_parallel_induct:
-  "n > 0 \<Longrightarrow> n \<le> N \<Longrightarrow>
-  \<lbrace>\<lambda>s0 s. plus2_inv {..< N} s \<and> (\<forall>i < N. threadv s i = 0) \<and> s = s0\<rbrace>,\<lbrace>plus2_rel {..< N} {..< n}\<rbrace>
-    fold parallel (map plus2_x [1 ..< n]) (plus2_x 0) \<lbrace>plus2_rel {..< N} ( - {..< n})\<rbrace>,\<lbrace>\<lambda>_ _ s.
-        plus2_inv {..< N} s \<and> (\<forall>i < n. threadv s i = 2)\<rbrace>"
+  "\<lbrakk>n > 0; n \<le> N\<rbrakk> \<Longrightarrow>
+   \<lbrace>\<lambda>s0 s. plus2_inv {..< N} s \<and> (\<forall>i < N. threadv s i = 0) \<and> s = s0\<rbrace>,\<lbrace>plus2_rel {..< N} {..< n}\<rbrace>
+   fold parallel (map plus2_x [1 ..< n]) (plus2_x 0)
+   \<lbrace>plus2_rel {..< N} ( - {..< n})\<rbrace>,\<lbrace>\<lambda>_ _ s. plus2_inv {..< N} s \<and> (\<forall>i < n. threadv s i = 2)\<rbrace>"
   apply (induct n)
    apply simp
   apply (case_tac n)
@@ -163,18 +166,19 @@ lemma plus2_x_n_parallel_induct:
    apply clarsimp
   apply (clarsimp split del: if_split)
   apply (rule rg_weaken_pre, rule rg_strengthen_post,
-    rule rg_validI, rule plus2_x_property[where tids="{..< N}"],
-    assumption, (clarsimp simp: plus2_rel_def)+)
+         rule rg_validI, rule plus2_x_property[where tids="{..< N}"], assumption,
+         (clarsimp simp: plus2_rel_def)+)
    apply (auto dest: less_Suc_eq[THEN iffD1])[1]
   apply clarsimp
   done
 
 theorem plus2_x_n_parallel:
   "n > 0 \<Longrightarrow>
-  \<lbrace>\<lambda>s0 s. mainv s = 0 \<and> (\<forall>i < n. threadv s i = 0) \<and> s = s0\<rbrace>,\<lbrace>plus2_rel {..< n} {..< n}\<rbrace>
-    fold parallel (map plus2_x [1 ..< n]) (plus2_x 0) \<lbrace>\<lambda>s0 s. True\<rbrace>,\<lbrace>\<lambda>_ _ s. mainv s = (n * 2)\<rbrace>"
+   \<lbrace>\<lambda>s0 s. mainv s = 0 \<and> (\<forall>i < n. threadv s i = 0) \<and> s = s0\<rbrace>,\<lbrace>plus2_rel {..< n} {..< n}\<rbrace>
+   fold parallel (map plus2_x [1 ..< n]) (plus2_x 0)
+   \<lbrace>\<lambda>s0 s. True\<rbrace>,\<lbrace>\<lambda>_ _ s. mainv s = (n * 2)\<rbrace>"
   apply (rule rg_weaken_pre, rule rg_strengthen_post,
-      rule rg_strengthen_guar, erule plus2_x_n_parallel_induct)
+         rule rg_strengthen_guar, erule plus2_x_n_parallel_induct)
      apply simp
     apply simp
    apply (clarsimp simp: plus2_inv_def)
@@ -182,8 +186,8 @@ theorem plus2_x_n_parallel:
   done
 
 lemma par_tr_fin_principle_parallel:
-  "par_tr_fin_principle f \<Longrightarrow> par_tr_fin_principle g
-    \<Longrightarrow> par_tr_fin_principle (parallel f g)"
+  "\<lbrakk>par_tr_fin_principle f; par_tr_fin_principle g\<rbrakk>
+   \<Longrightarrow> par_tr_fin_principle (parallel f g)"
   apply (subst par_tr_fin_principle_def, clarsimp simp: parallel_def3)
   apply (drule(1) par_tr_fin_principleD)+
   apply (clarsimp simp: neq_Nil_conv)
@@ -191,12 +195,12 @@ lemma par_tr_fin_principle_parallel:
 
 lemma fold_parallel_par_tr_fin_principle[where xs="rev xs" for xs, simplified]:
   "\<forall>x \<in> insert x (set xs). par_tr_fin_principle x
-    \<Longrightarrow> par_tr_fin_principle (fold parallel (rev xs) x)"
+   \<Longrightarrow> par_tr_fin_principle (fold parallel (rev xs) x)"
   by (induct xs, simp_all add: par_tr_fin_principle_parallel)
 
 lemma fold_parallel_prefix_closed[where xs="rev xs" for xs, simplified]:
   "\<forall>x \<in> insert x (set xs). prefix_closed x
-    \<Longrightarrow> prefix_closed (fold parallel (rev xs) x)"
+   \<Longrightarrow> prefix_closed (fold parallel (rev xs) x)"
   by (induct xs, simp_all add: prefix_closed_parallel)
 
 lemma bipred_disj_top_eq:
@@ -205,28 +209,29 @@ lemma bipred_disj_top_eq:
   by auto
 
 lemma fold_parallel_pfx_refn_induct:
-  "list_all2 (prefix_refinement sr sr sr (\<lambda>_ _. True) P Q (\<top>\<top>) (\<top>\<top>)) xs ys
-    \<Longrightarrow> prefix_refinement sr sr sr (\<lambda>_ _. True) P Q (\<top>\<top>) (\<top>\<top>) x y
-    \<Longrightarrow> \<forall>x \<in> set (x # xs). par_tr_fin_principle x
-    \<Longrightarrow> \<forall>y \<in> set (y # ys). prefix_closed y
-    \<Longrightarrow> prefix_refinement sr sr sr (\<lambda>_ _. True) P Q (\<top>\<top>) (\<top>\<top>)
-        (fold parallel (rev xs) x) (fold parallel (rev ys) y)"
+  "\<lbrakk>list_all2 (prefix_refinement sr sr sr (\<lambda>_ _. True) P Q (\<top>\<top>) (\<top>\<top>)) xs ys;
+    prefix_refinement sr sr sr (\<lambda>_ _. True) P Q (\<top>\<top>) (\<top>\<top>) x y;
+    \<forall>x \<in> set (x # xs). par_tr_fin_principle x;
+    \<forall>y \<in> set (y # ys). prefix_closed y\<rbrakk>
+   \<Longrightarrow> prefix_refinement sr sr sr (\<lambda>_ _. True) P Q (\<top>\<top>) (\<top>\<top>)
+         (fold parallel (rev xs) x) (fold parallel (rev ys) y)"
   apply (induct rule: list_all2_induct; simp)
   apply (rule prefix_refinement_parallel_triv[simplified bipred_disj_top_eq]; simp?)
    apply (clarsimp simp: fold_parallel_par_tr_fin_principle
                          fold_parallel_prefix_closed)+
   done
 
-lemmas fold_parallel_pfx_refn
-    = fold_parallel_pfx_refn_induct[where xs="rev xs" and ys="rev ys" for xs ys, simplified]
+lemmas fold_parallel_pfx_refn =
+  fold_parallel_pfx_refn_induct[where xs="rev xs" and ys="rev ys" for xs ys, simplified]
 
 theorem plus2_n_parallel:
-  "n > 0
-    \<Longrightarrow> \<lbrace>\<lambda>s0 s. s = 0 \<and> s = s0\<rbrace>,\<lbrace>\<lambda>a b. a = b\<rbrace>
-        fold parallel (replicate (n - 1) plus2) plus2 \<lbrace>\<lambda>s0 s. True\<rbrace>,\<lbrace>\<lambda>_ s0 s. s = n * 2\<rbrace>"
+  "n > 0 \<Longrightarrow>
+   \<lbrace>\<lambda>s0 s. s = 0 \<and> s = s0\<rbrace>,\<lbrace>\<lambda>a b. a = b\<rbrace>
+   fold parallel (replicate (n - 1) plus2) plus2
+   \<lbrace>\<lambda>s0 s. True\<rbrace>,\<lbrace>\<lambda>_ s0 s. s = n * 2\<rbrace>"
   apply (rule_tac sr="\<lambda>s t. t = mainv s" in prefix_refinement_validI)
       apply (rule prefix_refinement_weaken_rely,
-      rule_tac xs="map plus2_x [1 ..< n]" in fold_parallel_pfx_refn)
+             rule_tac xs="map plus2_x [1 ..< n]" in fold_parallel_pfx_refn)
            apply (clarsimp simp: list_all2_conv_all_nth)
            apply (rule pfx_refn_plus2_x)
           apply (rule pfx_refn_plus2_x[where tid=0])
